Defining impl PrecompileOutput

CoqOfRust/revm/revm_precompile/links/interface.v
@@ -25,14 +25,59 @@ Module PrecompileOutput.
   }.
 
   Global Instance IsLink : Link t := {
-    Φ := Ty.path "revm_precompile::PrecompileOutput";
+    Φ := Ty.path "revm_precompile::interface::PrecompileOutput";
     φ x :=
-        Value.StructRecord "revm_precompile::PrecompileOutput" [
+        Value.StructRecord "revm_precompile::interface::PrecompileOutput" [
           ("gas_used", φ x.(gas_used));
           ("bytes", φ x.(bytes))
         ];
     }.
 
-  
+    Definition of_ty : OfTy.t (Ty.path "revm_precompile::interface::PrecompileOutput").
+    Proof. eapply OfTy.Make with (A := t); reflexivity.
+    Defined.
+    Smpl Add apply of_ty : of_ty.
+
+    Lemma of_value_with gas_used gas_used' bytes bytes' :
+    gas_used' = φ gas_used ->
+    bytes' = φ bytes ->
+    Value.StructRecord "revm_precompile::interface::PrecompileOutput" [
+      ("gas_used", gas_used');
+      ("bytes", bytes')
+    ] = φ (Build_t gas_used bytes).
+  Proof. now intros; subst. Qed.
+  Smpl Add apply of_value_with : of_value.
+
+  Definition of_value (gas_used : U64.t) gas_used' (bytes : Bytes.t) bytes' :
+    gas_used' = φ gas_used ->
+    bytes' = φ bytes ->
+    OfValue.t (
+      Value.StructRecord "revm_precompile::interface::PrecompileOutput" [
+        ("gas_used", gas_used');
+        ("bytes", bytes')
+      ]
+    ).
+  Proof. econstructor; apply of_value_with; repeat eassumption.
+  Defined.
+  Smpl Add apply of_value : of_value.
 
 End PrecompileOutput.
+
+Module Impl_PrecompileOutput.
+  Definition Self : Set := PrecompileOutput.t.
+
+  (*
+     pub fn new(gas_used: u64, bytes: Bytes) -> Self {
+        Self { gas_used, bytes }
+    }
+  *)
+
+  Definition run_new 
+      (gas_used : U64.t) 
+      (bytes : Bytes.t)
+    : {{ interface.Impl_revm_precompile_interface_PrecompileOutput.new [] [] [φ gas_used; φ bytes] 🔽 PrecompileOutput.t }}.
+  Proof.
+    run_symbolic.
+  Defined.
+  Smpl Add apply run_new : run_closure.
+End Impl_PrecompileOutput.
